fix isep_assumption order, improve example, fix join rule

LLVM_DS_RBT/Load_Store_Example.thy
@@ -47,9 +47,9 @@ lemma example_correct:
   unfolding example_def
   supply map_leD[elim]
   apply vcg
-   apply vcg_compat
+  apply vcg_compat
   apply (isep_drule drule: value_ex_join_ent; join_filter) 
-  apply simp_all
+    apply simp_all
   apply sepE
   done
 
@@ -82,23 +82,40 @@ lemma example_correct_2:
 
 declare insert_opt_correct_ext'[vcg_rules del]
 
-definition "example2 t k1 v1 k2 v2 k3 f \<equiv>
+definition "example2 t k1 v1 k2 v2 k3 f1 f2 \<equiv>
   do {
     p \<leftarrow> lookup_ptr t k1;
     t' \<leftarrow> insert_opt k2 v2 t;
     vp \<leftarrow> load p;
     t'' \<leftarrow> delete_opt k3 t';
-    vp' \<leftarrow> f vp;
+    vp' \<leftarrow> f1 vp;
+    f2 v2;
     store p v1;
     return (t'', vp')
   }
 "
 
+lemma rbt_assn_ext_diff_ex_sets [fri_red_rules]:
+  "ex1 = ex2 \<Longrightarrow> is_sep_red \<box> \<box> (rbt_assn_ext t ex1 ti) (rbt_assn_ext t ex2 ti)"
+  apply (rule is_sep_redI)
+  apply simp
+  subgoal premises prems
+    apply (sep isep_dest: prems(2))
+    done
+  done
+
+
+lemma rbt_update_comp_comm: 
+  "k1 \<noteq> k2 \<Longrightarrow> rbt_update (rbt_update t k1 v1) k2 v2 = rbt_update (rbt_update t k2 v2) k1 v1" 
+  apply (induction t) by auto
+
+
 lemma example2_correct:
   assumes
-    [vcg_rules]: "\<And>v vi. llvm_htriple (\<upharpoonleft>value_assn v vi) (fi vi) (\<lambda>res_v. \<upharpoonleft>value_assn (f v) res_v)"
+    [vcg_rules]: "\<And>v vi. llvm_htriple (\<upharpoonleft>value_assn v vi) (f1i vi) (\<lambda>res_v. \<upharpoonleft>value_assn (f1 v) res_v)" and
+    [vcg_rules]: "\<And>v vi. llvm_htriple (\<upharpoonleft>value_assn v vi) (f2i vi) (\<lambda>_. \<upharpoonleft>value_assn (f2 v) vi)"
   shows
-  "is_rbt (rbt_of t) \<Longrightarrow> rbt_lookup (rbt_of t) k1 \<noteq> None \<Longrightarrow> k1 \<noteq> k3 \<Longrightarrow>
+    "\<lbrakk>is_rbt (rbt_of t); rbt_lookup (rbt_of t) k1 \<noteq> None; k1 \<noteq> k2; k1 \<noteq> k3; k2 \<noteq> k3\<rbrakk> \<Longrightarrow>
   llvm_htriple
   (
     rbt_assn_ext t {} ti **
@@ -108,12 +125,12 @@ lemma example2_correct:
     \<upharpoonleft>value_assn v1 v1i **
     \<upharpoonleft>value_assn v2 v2i
   )
-  (example2 ti k1i v1i k2i v2i k3i fi)
+  (example2 ti k1i v1i k2i v2i k3i f1i f2i)
   (\<lambda>(res_ti, res_vi). EXS res_t res_v.
     rbt_assn_ext res_t {} res_ti **
     \<upharpoonleft>key_assn k1 k1i ** \<upharpoonleft>key_assn k3 k3i **
-    \<upharpoonleft>value_assn (f (the (rbt_lookup (rbt_delete k3 (rbt_insert k2 v2 (rbt_of t))) k1))) res_vi **
-    \<up>(rbt_of res_t = (rbt_update (rbt_delete k3 (rbt_insert k2 v2 (rbt_of t))) k1 v1))
+    \<upharpoonleft>value_assn (f1 (the (rbt_lookup (rbt_delete k3 (rbt_insert k2 v2 (rbt_of t))) k1))) res_vi **
+    \<up>(rbt_of res_t = (rbt_update (rbt_update (rbt_delete k3 (rbt_insert k2 v2 (rbt_of t))) k1 v1)) k2 (f2 v2))
   )
   "
   unfolding example2_def
@@ -125,15 +142,32 @@ lemma example2_correct:
   apply vcg_rl
 
    apply vcg_compat
-   apply (sepwith auto)
+   apply (sepwith auto) 
+
+  apply vcg_solve
+  apply vcg
+  apply vcg_rl
+
+   apply vcg_compat
+   apply (sepwith \<open>solves auto\<close>)
+
 
   apply vcg_solve
   apply vcg
 
+
   apply vcg_compat
-  apply (sepEwith \<open>join_filter, auto?\<close> isep_dest: value_ex_join_ent)
-  apply simp 
-  apply sep
+  subgoal 
+    apply (sepEwith \<open>solves auto\<close> isep_dest: value_ex_join_ent) 
+
+    apply sep 
+
+    apply (simp add: rbt_update_comp_comm rbt_lookup_delete inv_12_def rbt_lookup_rbt_insert)
+
+    subgoal premises
+      apply entails_box_solver
+      done
+    done
   done
 
 end
