LLVM_DS_RBT/Extended_Assertion_Exceptions.thy
@@ -2,6 +2,7 @@ theory Extended_Assertion_Exceptions
   imports 
     Abstract_Rbt
     Assertion_Tree_Lookup
+    Utilities_Ext
 begin
 
 context rbt_impl
@@ -123,18 +124,24 @@ lemma value_ex_split_red:
     done
   done
 
-lemma value_ex_join_ent:
+lemma value_ex_join_ent':
   assumes
+    "value_of_key t ti kn = Some vi" and
     "kn \<in> ex" and
-    "value_of_key t1 ti kn = Some vi" and
-    "rbt_sorted (rbt_of t1)"
+    "rbt_sorted (rbt_of t)"
   shows
     "
-    rbt_assn_ext t1 ex ti ** \<upharpoonleft>value_assn v vi \<turnstile> 
-    (EXS t2. rbt_assn_ext t2 (ex - {kn}) ti ** \<up>(rbt_of t2 = rbt_update (rbt_of t1) kn v))
+    rbt_assn_ext t ex ti ** \<upharpoonleft>value_assn v vi \<turnstile> 
+    (EXS t_res.
+      rbt_assn_ext t_res (ex - {kn}) ti **
+      \<up>(rbt_of t_res = rbt_update (rbt_of t) kn v) **
+      ctx(rbt_sorted (rbt_of t_res)) **
+      \<up>(ptr_of_key t_res ti = ptr_of_key t ti) **
+      \<up>(value_of_key t_res ti = value_of_key t ti)
+    )
     "
   using assms
-proof (induction t1 arbitrary: ti)
+proof (induction t arbitrary: ti)
   case ATEmpty
   then show ?case unfolding value_of_key.simps by simp
 next
@@ -147,15 +154,27 @@ next
     from less have "kn \<noteq> k" by simp
     moreover from ATBranch(5) rbt_greater_trans less have "kn \<guillemotleft>| rbt_of r" by auto
 
-    ultimately show ?thesis using ATBranch(3-4) less
+    ultimately show ?thesis using ATBranch(3-5) less
       apply - 
       unfolding rbt_assn_ext_unfold
       apply (isep_drule drule: ATBranch(1))
-      using ATBranch(5) apply (auto simp add: value_of_key.simps)[3]
-      apply sepE
-       apply auto[]
-      apply auto[]
-      apply sep
+      apply (auto simp add: value_of_key.simps)[3]
+ 
+      apply (sepEwith \<open>(solves auto)?\<close>)
+       apply (simp add: rbt_map_entry_rbt_less rbt_map_entry_rbt_sorted)  
+
+      apply (sepEwith \<open>(solves auto)?\<close>)
+      subgoal by (simp add: ptr_of_key_simps)
+
+      apply (sepEwith \<open>(solves auto)?\<close>)
+      subgoal 
+        apply simp
+        apply prune_pure
+        apply vok_solver 
+        done
+
+      apply simp
+      apply (sepEwith \<open>(solves auto)?\<close>)
       done
   next
     case equal
@@ -163,6 +182,7 @@ next
       unfolding rbt_assn_ext_unfold
       apply -
       apply (sepEwith \<open>auto intro: rbt_less_trans rbt_greater_trans\<close>)
+       apply vok_solver
       apply (simp add: value_of_key.simps)
       apply sep
       done
@@ -174,18 +194,32 @@ next
     moreover from greater have "kn \<noteq> k" by simp
     moreover from ATBranch(5) rbt_less_trans greater have "rbt_of l |\<guillemotleft> kn" by auto
 
-    ultimately show ?thesis using ATBranch(3-4) greater
+    ultimately show ?thesis using ATBranch(3-5) greater
       apply - 
       unfolding rbt_assn_ext_unfold
-      apply (isep_drule drule: ATBranch(2)) 
-      using ATBranch(5) apply (auto simp add: order_less_not_sym value_of_key.simps)[3]
-      apply sepE
-       apply auto[]
-      apply auto[]
-      apply sep
+      apply (isep_drule drule: ATBranch(2))
+      apply (auto simp add: value_of_key.simps)[3]
+ 
+      apply (sepEwith \<open>(solves auto)?\<close>)
+       apply (simp add: rbt_map_entry_rbt_greater rbt_map_entry_rbt_sorted)  
+
+      apply (sepEwith \<open>(solves auto)?\<close>)
+      subgoal by (simp add: ptr_of_key_simps)
+
+      apply (sepEwith \<open>(solves auto)?\<close>)
+      subgoal 
+        apply simp
+        apply prune_pure
+        apply vok_solver 
+        done
+
+      apply simp
+      apply (sepEwith \<open>(solves auto)?\<close>)
       done
   qed
 qed
+
+lemmas value_ex_join_ent = value_ex_join_ent'[simplified ctx_def]
 
 lemma value_ex_join_red:
   "rbt_sorted (rbt_of t1) \<Longrightarrow> k \<in> ex \<Longrightarrow> k \<notin> ex' \<Longrightarrow> value_of_key t1 ti k = Some vi \<Longrightarrow>
